feat(rewriter): Add setAttributes, setProperties with GetSet lemmas
This adds setAttributes and setProperties to Rewriter/WfRewriter, with
corresponding GetSet lemmas for each.
This also adds the same proof about WellFormed for setProperties that already
exists for setAttributes.

The initial motivation for this was to remove the current sorrys in
setFunctionType (Reconciliation.lean).
This and other potential call sites will be updated in follow-ups to keep this
smaller.

Veir/Rewriter/WfRewriter/Basic.lean
@@ -152,6 +152,45 @@ def WfRewriter.replaceOperand! (wfCtx : WfIRContext OpInfo) (use : OpOperandPtr)
   else
     panic! "WfRewriter.replaceOperand! failed: operand use is out of bounds"
 
+/-- Set the attributes of an operation. -/
+@[inline]
+def WfRewriter.setAttributes (wfCtx : WfIRContext OpInfo) (op : OperationPtr) (newAttrs : DictionaryAttr)
+    (opIn : op.InBounds wfCtx.raw := by grind) : WfIRContext OpInfo :=
+  ⟨Rewriter.setAttributes wfCtx.raw op newAttrs opIn,
+    by grind [Rewriter.setAttributes_WellFormed]⟩
+
+/-- Set the attributes of an operation, panicking if the operation is out of bounds. -/
+def WfRewriter.setAttributes! (wfCtx : WfIRContext OpInfo) (op : OperationPtr) (newAttrs : DictionaryAttr)
+    : WfIRContext OpInfo :=
+  if hop : op.InBounds wfCtx.raw then
+    WfRewriter.setAttributes wfCtx op newAttrs hop
+  else
+    panic! "WfRewriter.replaceOperand! failed: operation is out of bounds"
+
+/-- Set the properties of an operation. -/
+@[inline]
+def WfRewriter.setProperties {opCode : OpInfo} (wfCtx : WfIRContext OpInfo) (op : OperationPtr)
+    (newProps : HasOpInfo.propertiesOf opCode)
+    (opIn : op.InBounds wfCtx.raw := by grind)
+    (hprop : op.getOpType! wfCtx.raw = opCode := by grind) :
+    WfIRContext OpInfo :=
+  ⟨Rewriter.setProperties wfCtx.raw op newProps opIn hprop,
+    by grind [Rewriter.setProperties_WellFormed]⟩
+
+/--
+Set the properties of an operation, panicking if the operation is out of bounds, or if the
+property types don't match.
+-/
+def WfRewriter.setProperties! {opCode : OpInfo} (wfCtx : WfIRContext OpInfo) (op : OperationPtr)
+    (newProperties : HasOpInfo.propertiesOf opCode) : WfIRContext OpInfo :=
+  if opIn : op.InBounds wfCtx.raw then
+    if hprop : op.getOpType! wfCtx.raw = opCode then
+      WfRewriter.setProperties wfCtx op newProperties opIn hprop
+    else
+      panic! "WfRewriter.setProperties! failed: property types don't match"
+  else
+    panic! "WfRewriter.setProperties! failed: operation is out of bounds"
+
 /-- Set the type of a value. -/
 @[inline]
 def WfRewriter.setType (wfCtx : WfIRContext OpInfo) (value : ValuePtr) (newType : TypeAttr)
